only one problem left for cont spsStep #108

untimed/SpsStep.thy
@@ -6,41 +6,35 @@ begin
 
 default_sort type
 type_synonym 'm SPS = "'m SPF uspec"
-  
+    
 definition spsStep_h::"((channel\<rightharpoonup>'m::message) \<Rightarrow> 'm SPS)\<rightarrow> ((channel\<rightharpoonup>'m::message) \<Rightarrow> 'm SPF) set rev"where
-"spsStep_h= (\<Lambda> h. setify\<cdot>(\<lambda>e. fst(Rep_uspec(h e))))"
+"spsStep_h= (\<Lambda> h. setify\<cdot>(\<lambda>e. uspecRevSet\<cdot>(h e)))"
 
-lemma spsStep_h_mono[simp]:"monofun (\<lambda> h::((channel\<rightharpoonup>'m::message) \<Rightarrow> 'm SPS). setify\<cdot>(\<lambda>e. fst(Rep_uspec(h e))))"
-proof(rule monofunI)
+lemma spsStep_h_mono[simp]:"monofun (\<lambda> h::((channel\<rightharpoonup>'m::message) \<Rightarrow> 'm SPS). setify\<cdot>(\<lambda>e. uspecRevSet\<cdot>(h e)))"
+proof(rule monofunI, simp add: uspecRevSet_def)
   fix x y::"(channel \<Rightarrow> 'm::message option) \<Rightarrow> 'm SPS"
   assume a1:"x \<sqsubseteq> y"
   then show "setify\<cdot>(\<lambda>e. fst (Rep_uspec (x e))) \<sqsubseteq> setify\<cdot>(\<lambda>e. fst (Rep_uspec (y e)))"
     by (simp add: below_fun_def fst_monofun monofun_cfun_arg rep_uspec_belowI)
 qed
    
-lemma spsStep_h_cont[simp]:"cont (\<lambda> h::((channel\<rightharpoonup>'m::message) \<Rightarrow> 'm SPS). setify\<cdot>(\<lambda>e. fst(Rep_uspec(h e))))"
+lemma spsStep_h_cont[simp]:"cont (\<lambda> h::((channel\<rightharpoonup>'m::message) \<Rightarrow> 'm SPS). setify\<cdot>(\<lambda>e. uspecRevSet\<cdot>(h e)))"
 proof(rule Cont.contI2,simp)
   fix Y::"nat \<Rightarrow> (channel \<Rightarrow> 'm::message option) \<Rightarrow> 'm SPS"
   assume a1:"chain Y"
-  assume a2:"chain (\<lambda>i::nat. setify\<cdot>(\<lambda>e. fst (Rep_uspec (Y i e))))"
-  have a3:"\<forall>e. (\<Squnion>i. Y i) e = (\<Squnion>i. Y i e)"
-    by (simp add: a1 lub_fun)
-  have a4:"\<forall>e. (Rep_uspec (\<Squnion>i. Y i e)) = (\<Squnion>i. (Rep_uspec ( Y i e)))"
-    by (metis a1 ch2ch_fun cont2contlubE uspec_rep_cont)
-  have a5:"\<forall>e. fst (\<Squnion>i. (Rep_uspec ( Y i e))) = (\<Squnion>i. fst (Rep_uspec ( Y i e)))"
-    by (smt a1 a4 ch2ch_fun contlub_cfun_arg lub_eq uspecrevset_insert)
-  have a6:" (\<lambda>e. (\<Squnion>i. fst (Rep_uspec ( Y i e)))) = (\<Squnion>i. (\<lambda>e. fst (Rep_uspec ( Y i e))))"
-    apply(subst lub_fun, auto)
-    by (metis (mono_tags, lifting) a1 fst_monofun fun_below_iff po_class.chain_def rep_uspec_belowI)
-  show "setify\<cdot>(\<lambda>e. fst (Rep_uspec ((\<Squnion>i. Y i) e))) \<sqsubseteq> (\<Squnion>i. setify\<cdot>(\<lambda>e. fst (Rep_uspec (Y i e))))"
-    apply(simp add: a1 lub_fun a2 a4 a5 a6)
-    apply(subst contlub_cfun_arg)
-    apply (metis (mono_tags, lifting) a1 below_fun_def fst_monofun po_class.chain_def rep_uspec_belowI)
-    by simp
+  assume a2:"chain (\<lambda>i::nat. setify\<cdot>(\<lambda>e::channel \<Rightarrow> 'm option. uspecRevSet\<cdot>(Y i e)))"
+  have a3:"(\<lambda>e. \<Squnion>i. uspecRevSet\<cdot>(Y i e)) =  (\<Squnion>i.(\<lambda>e. uspecRevSet\<cdot>(Y i e)))"
+    apply(subst lub_fun,auto)
+    by (metis (mono_tags, lifting) a1 cont_pref_eq1I fun_below_iff po_class.chain_def)
+  show "setify\<cdot>(\<lambda>e. uspecRevSet\<cdot>((\<Squnion>i::nat. Y i) e)) \<sqsubseteq> (\<Squnion>i. setify\<cdot>(\<lambda>e. uspecRevSet\<cdot>(Y i e)))"
+    apply(simp add: a1 lub_fun)
+    apply (simp add: contlub_cfun_arg a1 ch2ch_fun a3)
+    apply(subst contlub_cfun_arg, auto)
+    by (metis (mono_tags, lifting) a1 fun_below_iff monofun_cfun_arg po_class.chain_def)
 qed
   
 
-lemma spsStep_h_insert:"spsStep_h\<cdot>f = setify\<cdot>(\<lambda>e. fst(Rep_uspec(f e)))"
+lemma spsStep_h_insert:"spsStep_h\<cdot>f = setify\<cdot>(\<lambda>e. uspecRevSet\<cdot>(f e))"
   by(simp add: spsStep_h_def)
     
 (* like spfStep, copy & pasteonly on SPS *)
@@ -73,12 +67,19 @@ proof(rule monofunI)
        Abs_rev_uspec {spfStep In Out\<cdot>g |g. g \<in> inv Rev (spsStep_h\<cdot>y)} In Out"
     by (metis (no_types, lifting) Pair_below_iff below_refl below_rev.simps below_uspec_def h1 h2 h3 rep_abs_uspec)
 qed
-  
+ 
+lemma uspec_lub_insert:assumes "chain (Y::nat \<Rightarrow> 'm::ufuncl set rev)" shows "(\<Squnion>i. (Y i, Discr In, Discr Out)) = ((\<Squnion>i. Y i), Discr In, Discr Out)"
+  sorry
+
 lemma spsStep_cont[simp]:assumes "finite In" shows"cont (\<lambda>h. Abs_rev_uspec {spfStep In Out\<cdot>g | g. g \<in>inv Rev (spsStep_h\<cdot>h)} In Out)"
 proof(rule Cont.contI2, simp)
   fix Y::"nat \<Rightarrow> ((channel \<Rightarrow> 'a option) \<Rightarrow> 'a SPS)"
   assume a1:"chain Y"
   assume a2:"chain (\<lambda>i. Abs_rev_uspec {spfStep In Out\<cdot>g |g. g \<in> inv Rev (spsStep_h\<cdot>(Y i))} In Out)"
+  have a3:"chain (\<lambda>i::nat. setify\<cdot>(\<lambda>e. uspecRevSet\<cdot>(Y i e)))"
+    by (metis (mono_tags, lifting) a1 fun_below_iff monofun_cfun_arg po_class.chain_def)
+  have a4:"chain (\<lambda>i::nat. Rev {spfStep In Out\<cdot>g |g. g \<in> inv Rev (setify\<cdot>(\<lambda>e. uspecRevSet\<cdot>(Y i e)))})"
+    by (smt Collect_mono SetPcpo.less_set_def a3 below_rev.elims(2) below_rev.simps inv_rev_rev po_class.chain_def subsetCE)
   have h1:"\<forall>i. uspecWell (Rev {spfStep In Out\<cdot>g |g. g \<in> inv Rev (spsStep_h\<cdot>(Y i))}) (Discr In) (Discr Out)"
     by (smt finite mem_Collect_eq spfstep_dom spfstep_ran ufclDom_ufun_def ufclRan_ufun_def uspecWell.simps)
   have h2:"uspecWell (Rev {spfStep In Out\<cdot>g |g::(channel \<Rightarrow> 'a option) \<Rightarrow> ('a stream\<^sup>\<Omega>) ufun. g \<in> inv Rev (\<Squnion>i::nat. spsStep_h\<cdot>(Y i))}) (Discr In) (Discr Out)"
@@ -86,12 +87,49 @@ proof(rule Cont.contI2, simp)
   have h3:"Rep_uspec (Abs_uspec (\<Squnion>i::nat. (Rev {spfStep In Out\<cdot>g |g::(channel \<Rightarrow> 'a option) \<Rightarrow> ('a stream\<^sup>\<Omega>) ufun. g \<in> inv Rev (spsStep_h\<cdot>(Y i))}, Discr In, Discr Out)))
         =  (\<Squnion>i::nat. (Rev {spfStep In Out\<cdot>g |g::(channel \<Rightarrow> 'a option) \<Rightarrow> ('a stream\<^sup>\<Omega>) ufun. g \<in> inv Rev (spsStep_h\<cdot>(Y i))}, Discr In, Discr Out))"
     by (metis (mono_tags, lifting) a2 cont2contlubE h1 lub_eq lub_uspec rep_abs_uspec uspec_rep_cont)
-  have h4:"chain (\<lambda>i::nat. Rev {g. \<forall>m. g m \<in> Rep_rev_uspec (Y i m)})"
-    by (smt Collect_mono SetPcpo.less_set_def a1 below_fun_def below_rev.elims(2) below_rev.simps fst_monofun inv_rev_rev po_class.chain_def rep_uspec_belowI subsetCE) 
-  have h5:"(\<Squnion>i. (Rev {spfStep In Out\<cdot>g |g. \<forall>m. g m \<in> Rep_rev_uspec (Y i m)}, Discr In, Discr Out)) = ((\<Squnion>i. Rev{spfStep In Out\<cdot>g |g. \<forall>m. g m \<in> Rep_rev_uspec (Y i m)}), Discr In, Discr Out )"
-    sorry
-  have h6:"chain (\<lambda>i::nat. Rev {spfStep In Out\<cdot>g |g::(channel \<Rightarrow> 'a option) \<Rightarrow> ('a stream\<^sup>\<Omega>) ufun. \<forall>m::channel \<Rightarrow> 'a option. g m \<in> Rep_rev_uspec (Y i m)})"
-    by (smt Collect_mono SetPcpo.less_set_def a1 below_rev.elims(2) below_rev.simps fst_monofun fun_below_iff inv_rev_rev po_class.chain_def rep_uspec_belowI subsetCE)
+  have h4:"\<And>x.
+       \<forall>xa.
+          (\<exists>i. xa = {spfStep In Out\<cdot>g |g. g \<in> inv Rev (setify\<cdot>(\<lambda>e. uspecRevSet\<cdot>(Y i e)))}) \<longrightarrow> x \<in> xa \<Longrightarrow>
+       \<exists>g. x = spfStep In Out\<cdot>g \<and>
+          (\<forall>x. (\<exists>i. x = inv Rev (setify\<cdot>(\<lambda>e. uspecRevSet\<cdot>(Y i e)))) \<longrightarrow> g \<in> x)"
+  proof-
+    fix x::"'a SPF"
+    have h1:"(\<forall>xa.
+          (\<exists>i. xa = {spfStep In Out\<cdot>g |g. g \<in> inv Rev (setify\<cdot>(\<lambda>e. uspecRevSet\<cdot>(Y i e)))}) \<longrightarrow> x \<in> xa) = (\<forall>i. x\<in>{spfStep In Out\<cdot>g |g. g \<in> inv Rev (setify\<cdot>(\<lambda>e. uspecRevSet\<cdot>(Y i e)))})"
+      by auto
+    have h2:"(\<exists>g. x = spfStep In Out\<cdot>g \<and> (\<forall>x. (\<exists>i. x = inv Rev (setify\<cdot>(\<lambda>e. uspecRevSet\<cdot>(Y i e)))) \<longrightarrow> g \<in> x)) = (\<exists>g. x = spfStep In Out\<cdot>g \<and> (\<forall>i. g\<in> inv Rev (setify\<cdot>(\<lambda>e. uspecRevSet\<cdot>(Y i e)))))"
+      by auto
+    have "(\<forall>i. \<exists>g.  (\<forall>m. g m \<in> Rep_rev_uspec (Y i m)) \<and> x = spfStep In Out\<cdot>g) =  (\<exists>g.\<forall>i.  (\<forall>m. g m \<in> Rep_rev_uspec (Y i m)) \<and> x = spfStep In Out\<cdot>g)"
+    proof(auto)
+      assume a1:"\<forall>i::nat. \<exists>g::(channel \<Rightarrow> 'a option) \<Rightarrow> ('a stream\<^sup>\<Omega>) ufun. (\<forall>m::channel \<Rightarrow> 'a option. g m \<in> Rep_rev_uspec (Y i m)) \<and> x = spfStep In Out\<cdot>g"
+      obtain g where g_def:"\<exists>i. (\<forall>m. g m \<in> Rep_rev_uspec (Y i m)) \<and> x = spfStep In Out\<cdot>g"
+        using a1 by blast(*
+      have problem:"\<And>u w x. ufRestrict In Out\<cdot>(u x) = (u x) \<Longrightarrow> ufRestrict In Out\<cdot>(w x) = (w x) \<Longrightarrow>  spfStep In Out\<cdot>u = spfStep In Out\<cdot>w \<Longrightarrow> u=w"
+        sorry*)
+      have h1:"(\<forall>i m. g m \<in> Rep_rev_uspec (Y i m)) \<and> x = spfStep In Out\<cdot>g"
+      proof(cases "\<exists>i m. uspecDom\<cdot>(Y i m) \<noteq>In \<or> uspecRan\<cdot>(Y i m) \<noteq>Out")
+        case True
+        then show ?thesis sorry
+      next
+        case False
+        then show ?thesis sorry
+      qed
+      then show "\<exists>g. (\<forall>i m. g m \<in> Rep_rev_uspec (Y i m)) \<and> x = spfStep In Out\<cdot>g"
+        by blast
+    qed
+    then have h3_h:"\<forall>i. \<exists>g.  (\<forall>m. g m \<in> Rep_rev_uspec (Y i m)) \<and> x = spfStep In Out\<cdot>g \<Longrightarrow>
+    \<exists>g.  (\<forall>i m. g m \<in> Rep_rev_uspec (Y i m)) \<and> x = spfStep In Out\<cdot>g"
+      by simp
+    have h3:"\<forall>i. \<exists>g. x = spfStep In Out\<cdot>g \<and> g \<in> inv Rev (setify\<cdot>(\<lambda>e. uspecRevSet\<cdot>(Y i e))) \<Longrightarrow>
+    \<exists>g. x = spfStep In Out\<cdot>g \<and> (\<forall>i. g \<in> inv Rev (setify\<cdot>(\<lambda>e. uspecRevSet\<cdot>(Y i e))))"
+      apply(simp add: setify_def inv_rev_rev uspecrevset_insert) using h3_h by blast
+    show"\<forall>xa.
+          (\<exists>i. xa = {spfStep In Out\<cdot>g |g. g \<in> inv Rev (setify\<cdot>(\<lambda>e. uspecRevSet\<cdot>(Y i e)))}) \<longrightarrow> x \<in> xa \<Longrightarrow>
+       \<exists>g.
+          x = spfStep In Out\<cdot>g \<and>
+          (\<forall>x. (\<exists>i. x = inv Rev (setify\<cdot>(\<lambda>e. uspecRevSet\<cdot>(Y i e)))) \<longrightarrow> g \<in> x)"
+    by(simp add: h1 h2 h3)
+  qed
   show "Abs_rev_uspec {spfStep In Out\<cdot>g |g. g \<in> inv Rev (spsStep_h\<cdot>(\<Squnion>i. Y i))} In Out \<sqsubseteq>
        (\<Squnion>i. Abs_rev_uspec {spfStep In Out\<cdot>g |g. g \<in> inv Rev (spsStep_h\<cdot>(Y i))} In Out)"
     apply(simp add: a1 contlub_cfun_fun contlub_cfun_arg)
@@ -100,14 +138,11 @@ proof(rule Cont.contI2, simp)
     apply(simp add: lub_uspec a2)
     apply(simp only: h1 rep_abs_uspec h3)
     apply(simp add: a1 spsStep_h_insert)
-    apply(simp add: setify_def inv_rev_rev h5)
-    apply(subst setrevLubEqInterII, simp add: h4)
-    apply(subst setrevLubEqInter, simp add: h6 ,simp add:inv_rev_rev rev_inv_rev)
-    apply(simp add: less_set_def)
-    apply(simp add: assms spfstep_insert)
-    apply auto 
-    apply(simp add: assms spfstep_insert)
-    sorry
+    apply(simp add: setrevLubEqInterII a3)
+    apply(simp add: uspec_lub_insert setrevLubEqInter a4)
+    apply(simp add: less_set_def inv_rev_rev rev_inv_rev)
+    apply auto
+    by(simp add: h4)
 qed
   
 end
